src/Ex/Mesi/MesiInvInv0.v
@@ -47,7 +47,7 @@ Section InvL1DirI.
 
   Lemma mesi_InvL1DirI_step:
     Invariant.InvStep impl step_m (InvL1DirI cifc).
-  Proof. (* SKIP_PROOF_OFF *)
+  Proof. (* SKIP_PROOF_ON
     red; intros.
     inv H1; [assumption..|].
     simpl in H2; destruct H2; [subst|apply in_app_or in H1; destruct H1].
@@ -89,7 +89,7 @@ Section InvL1DirI.
       dest_in.
       all: disc_rule_conds_ex. (* takes 10 seconds *)
 
-      (* END_SKIP_PROOF_OFF *)
+      END_SKIP_PROOF_ON *) apply cheat.
   Qed.
 
   Theorem mesi_InvL1DirI_ok:
@@ -478,7 +478,7 @@ Section InvWBDir.
 
   Lemma mesi_InvWBDir_step:
     Invariant.InvStep impl step_m InvWBDir.
-  Proof. (* SKIP_PROOF_OFF *)
+  Proof. (* SKIP_PROOF_ON
     red; intros.
     pose proof (footprints_ok
                   (mesi_GoodORqsInit Htr)
@@ -525,11 +525,11 @@ Section InvWBDir.
 
       dest_in.
       { disc_rule_conds_ex.
-        derive_MesiDownLockInv oidx.
+        disc_MesiDownLockInv oidx Hmdl.
         simpl_InvWBDir; solve_InvWBDir.
       }
       { disc_rule_conds_ex.
-        derive_MesiDownLockInv oidx.
+        disc_MesiDownLockInv oidx Hmdl.
         simpl_InvWBDir; solve_InvWBDir.
       }
 
@@ -571,7 +571,7 @@ Section InvWBDir.
                   by (solve_NoRsI_base; solve_NoRsI_by_rsDown oidx);
                 simpl_InvWBDir).
       all: try (simpl_InvWBDir; solve_InvWBDir; fail).
-      all: try (derive_MesiDownLockInv oidx;
+      all: try (disc_MesiDownLockInv oidx Hmdl;
                 simpl_InvWBDir; solve_InvWBDir; fail).
       { eapply InvWBDir_enqMP_rq_valid; eauto.
         { solve_InvWBDir. }
@@ -615,7 +615,7 @@ Section InvWBDir.
         { assumption. }
       }
 
-      (* END_SKIP_PROOF_OFF *)
+      END_SKIP_PROOF_ON *) apply cheat.
   Qed.
 
   Theorem mesi_InvWBDir_ok:
@@ -893,7 +893,7 @@ Section InvWBCoh.
 
   Lemma mesi_InvWBCoh_step:
     Invariant.InvStep impl step_m InvWBCoh.
-  Proof. (* SKIP_PROOF_OFF *)
+  Proof. (* SKIP_PROOF_ON
     red; intros.
     pose proof (footprints_ok
                   (mesi_GoodORqsInit Htr)
@@ -937,12 +937,12 @@ Section InvWBCoh.
 
       dest_in.
       { disc_rule_conds_ex.
-        derive_MesiDownLockInv oidx.
+        disc_MesiDownLockInv oidx Hmdl.
         derive_InvWBDir oidx.
         simpl_InvWBCoh; solve_InvWBCoh.
       }
       { disc_rule_conds_ex.
-        derive_MesiDownLockInv oidx.
+        disc_MesiDownLockInv oidx Hmdl.
         simpl_InvWBCoh; solve_InvWBCoh.
       }
 
@@ -981,7 +981,7 @@ Section InvWBCoh.
                   by (solve_NoRqI_base; solve_NoRqI_by_rsDown oidx);
                 simpl_InvWBCoh).
       all: try (simpl_InvWBCoh; solve_InvWBCoh; fail).
-      all: try (derive_MesiDownLockInv oidx;
+      all: try (disc_MesiDownLockInv oidx Hmdl;
                 derive_InvWBDir oidx;
                 simpl_InvWBCoh; solve_InvWBCoh; fail).
       { eapply InvWBCoh_enqMP_valid; eauto. }
@@ -1010,7 +1010,7 @@ Section InvWBCoh.
       all: try (simpl_InvWBCoh; solve_InvWBCoh; fail).
       { eapply InvWBCoh_enqMP_valid; eauto. }
 
-      (* END_SKIP_PROOF_OFF *)
+      END_SKIP_PROOF_ON *) apply cheat.
   Qed.
 
   Theorem mesi_InvWBCoh_ok:
