src/Ex/Mesi/MesiObjInv.v
@@ -1,0 +1,92 @@
+Require Import Bool List String Peano_dec Lia.
+Require Import Common FMap IndexSupport HVector Syntax Topology Semantics SemFacts StepM.
+Require Import Invariant TrsInv Simulation Serial SerialFacts.
+Require Import RqRsLangEx RqRsCorrect.
+
+Require Import Ex.Spec Ex.SpecInds Ex.Template.
+Require Import Ex.Mesi Ex.Mesi.Mesi.
+
+Set Implicit Arguments.
+
+Import PropMonadNotations.
+Import CaseNotations.
+
+Local Open Scope list.
+Local Open Scope hvec.
+Local Open Scope fmap.
+
+Existing Instance Mesi.ImplOStateIfc.
+
+Section ObjInv.
+  Variable topo: DTree.
+
+  Definition MesiUpLockObjInv (oidx: IdxT): ObjInv :=
+    fun ost orq =>
+      (rqiu <+- orq@[upRq];
+      rmsg <+- rqiu.(rqi_msg);
+      match case rmsg.(msg_id) on idx_dec default True with
+      | mesiRqS:
+          ost#[owned] = false /\ ost#[status] <= mesiI /\
+          ost#[dir].(dir_st) <= mesiS
+      | mesiRqM:
+          ost#[owned] = false /\ ost#[status] <= mesiS /\
+          ost#[dir].(dir_st) <= mesiS
+      end).
+
+  Definition DownLockFromChild (oidx: IdxT) (rqid: RqInfo Msg) :=
+    exists cidx,
+      rqid.(rqi_midx_rsb) = Some (downTo cidx) /\
+      parentIdxOf topo cidx = Some oidx.
+
+  Definition DownLockFromParent (oidx: IdxT) (rqid: RqInfo Msg) :=
+    rqid.(rqi_midx_rsb) = Some (rsUpFrom oidx).
+
+  Definition MesiDownLockObjInv (oidx: IdxT): ObjInv :=
+    fun ost orq =>
+      (rqid <+- orq@[downRq];
+      rmsg <+- rqid.(rqi_msg);
+      match case rmsg.(msg_id) on idx_dec default True with
+      | mesiRqS: DownLockFromChild oidx rqid /\
+                 ost#[status] <= mesiI /\ mesiE <= ost#[dir].(dir_st) <= mesiM /\
+                 In ost#[dir].(dir_excl) (subtreeChildrenIndsOf topo oidx) /\
+                 rqid.(rqi_minds_rss) = [rsUpFrom ost#[dir].(dir_excl)]
+      | mesiRqM: DownLockFromChild oidx rqid /\
+                 ost#[status] <= mesiS /\
+                 ((ost#[owned] = true /\ ost#[dir].(dir_st) = mesiS /\
+                   SubList ost#[dir].(dir_sharers) (subtreeChildrenIndsOf topo oidx) /\
+                   rqid.(rqi_minds_rss) = map rsUpFrom ost#[dir].(dir_sharers)) \/
+                  (mesiE <= ost#[dir].(dir_st) <= mesiM /\
+                   In ost#[dir].(dir_excl) (subtreeChildrenIndsOf topo oidx) /\
+                   rqid.(rqi_minds_rss) = [rsUpFrom ost#[dir].(dir_excl)]))
+      | mesiDownRqS: DownLockFromParent oidx rqid /\
+                     ost#[status] <= mesiI /\ mesiE <= ost#[dir].(dir_st) <= mesiM /\
+                     In ost#[dir].(dir_excl) (subtreeChildrenIndsOf topo oidx) /\
+                     rqid.(rqi_minds_rss) = [rsUpFrom ost#[dir].(dir_excl)]
+      | mesiDownRqI: DownLockFromParent oidx rqid /\
+                     ((ost#[dir].(dir_st) = mesiS /\
+                       SubList ost#[dir].(dir_sharers) (subtreeChildrenIndsOf topo oidx) /\
+                       rqid.(rqi_minds_rss) = map rsUpFrom ost#[dir].(dir_sharers)) \/
+                      (mesiE <= ost#[dir].(dir_st) <= mesiM /\
+                       In ost#[dir].(dir_excl) (subtreeChildrenIndsOf topo oidx) /\
+                       rqid.(rqi_minds_rss) = [rsUpFrom ost#[dir].(dir_excl)]))
+      end).
+
+  Definition MesiObjInvs (oidx: IdxT): ObjInv :=
+    fun ost orq =>
+      MesiUpLockObjInv oidx ost orq /\
+      MesiDownLockObjInv oidx ost orq.
+
+End ObjInv.
+
+Ltac disc_mesi_obj_invs :=
+  repeat
+    match goal with
+    | [H: MesiObjInvs _ _ _ _ |- _] => destruct H
+    | [H: MesiUpLockObjInv _ _ _ |- _] =>
+      red in H; mred; simpl in H; disc_rule_conds_const
+    | [H: MesiDownLockObjInv _ _ _ _ |- _] =>
+      red in H; mred; simpl in H; disc_rule_conds_const
+    | [Hmsg: msg_id ?rmsg = _, H: context [msg_id ?rmsg] |- _] =>
+      rewrite Hmsg in H; simpl in H
+    end.
+
